coq/Progress.v
@@ -8,6 +8,7 @@ do_while
 unary/binary ops
 argument objects
 
+Monadic constructors.
 
 === Requires big changes (Daniele)
 
